WIP

code/ecdsa/Hacl.Impl.EC.Core.fst
@@ -112,42 +112,6 @@ let isPointAtInfinityPrivate #c p =
     (as_nat c h0 (gsub p (2ul *! len) len)); 
   r
 
-
-val lemma_norm_as_specification: #c: curve 
-  -> xD: nat {xD < getPrime c} 
-  -> yD: nat {yD < getPrime c} 
-  -> zD: nat {zD < getPrime c} -> 
-  x3 : nat {x3 == xD * (pow (zD * zD) (getPrime c - 2) % getPrime c) % getPrime c}-> 
-  y3 : nat {y3 == yD * (pow (zD * zD * zD) (getPrime c -2) % getPrime c) % getPrime c} -> 
-  z3 : nat {if isPointAtInfinity(xD, yD, zD) then z3 == 0 else z3 == 1} -> 
-  Lemma (
-    let (xN, yN, zN) = _norm #c (xD, yD, zD) in 
-    x3 == xN /\ y3 == yN /\ z3 == zN)
-
-
-let lemma_norm_as_specification #c xD yD zD x3 y3 z3 = 
-  let prime = getPrime c in 
-
-  calc (==)
-  {
-    xD * (pow (zD * zD) (getPrime c - 2) % prime) % prime;
-    (==) {}
-    xD * (modp_inv2_pow #c (zD * zD)) % prime;
-    (==) {_ by (canon())}
-    modp_inv2_pow #c (zD * zD) * xD % prime;
-  };
-
-  calc (==)
-  {
-    yD * (pow (zD * zD * zD) (getPrime c -2) % prime) % prime;
-    (==) {}
-    yD * (modp_inv2_pow #c (zD * zD * zD)) % prime;
-    (==) {_ by (canon())}
-    modp_inv2_pow #c (zD * zD * zD) * yD % prime;
-  };
-  admit()
-
-
 val normalisation_update: #c: curve -> z2x: felem c -> z3y: felem c -> p: point c -> resultPoint: point c -> 
   Stack unit 
   (requires fun h -> live h z2x /\ live h z3y /\ live h resultPoint /\ live h p /\ 
@@ -249,8 +213,7 @@ let norm #c p resultPoint tempBuffer =
     let h1 = ST.get() in 
 
   lemma_norm #c
-    (fromDomainPoint #c #DH (point_prime_to_coordinates c (as_seq h0 p))) 
-    (point_prime_to_coordinates c (as_seq h1 resultPoint))
+    (fromDomainPoint #c #DH (point_as_nat c h0 p)) (point_as_nat c h1 resultPoint)
 
 
 let normX #c p result tempBuffer = 
@@ -258,12 +221,9 @@ let normX #c p result tempBuffer =
   let len = getCoordinateLenU64 c in 
   
   let xf = sub p (size 0) len in 
-  let yf = sub p len len in 
   let zf = sub p (size 2 *! len) len in 
   
   let z2f = sub tempBuffer len len in 
-  let z3f = sub tempBuffer (size 2 *! len) len in
-
   let t8 = sub tempBuffer (3ul *. len) (8ul *. len) in 
 
     let h0 = ST.get() in 
@@ -272,38 +232,37 @@ let normX #c p result tempBuffer =
   montgomery_multiplication_buffer_dh #c z2f xf z2f; 
   fromDomain z2f result;
 
+  
     let prime = getPrime c in 
-    power_distributivity (fromDomain_ #c #DH (as_nat c h0 zf) * fromDomain_ #c #DH (as_nat c h0 zf)) (prime - 2) prime
+
+    let xD = fromDomain_ #c #DH (as_nat c h0 xf) in 
+    let zD = fromDomain_ #c #DH (as_nat c h0 zf) in 
+    
+    calc (==)
+    {
+      (pow (zD * zD % prime) (prime - 2) % prime) * xD % prime;
+      (==) {lemma_pow_mod_n_is_fpow prime (zD * zD % prime) (prime - 2)}
+      (modp_inv2 #c (zD * zD)) * xD % prime;
+    }  
 
 
-val lemma_point_to_domain: #c: curve ->  h0: mem -> h1: mem 
-  ->  p: point c 
-  -> result: point c ->  Lemma
-   (requires (
-     point_x_as_nat c h0 p < getPrime c /\ 
-     point_y_as_nat c h0 p < getPrime c /\
-     point_z_as_nat c h0 p < getPrime c /\
-       point_x_as_nat c h1 result == toDomain_ #c #DH (point_x_as_nat c h0 p) /\
-       point_y_as_nat c h1 result == toDomain_ #c #DH (point_y_as_nat c h0 p) /\
-       point_z_as_nat c h1 result == toDomain_ #c #DH (point_z_as_nat c h0 p) 
-     )
-   )
-   (ensures (fromDomainPoint #c #DH (point_prime_to_coordinates c (as_seq h1 result)) == point_prime_to_coordinates c (as_seq h0 p)))
+val lemma_point_to_domain: #c: curve ->  h0: mem -> h1: mem ->  p: point c -> result: point c ->
+  Lemma (requires (point_eval c h0 p /\ point_eval c h1 result /\
+    point_x_as_nat c h1 result == toDomain_ #c #DH (point_x_as_nat c h0 p) /\
+    point_y_as_nat c h1 result == toDomain_ #c #DH (point_y_as_nat c h0 p) /\
+    point_z_as_nat c h1 result == toDomain_ #c #DH (point_z_as_nat c h0 p)))
+   (ensures (fromDomainPoint #c #DH (point_as_nat c h1 result) == point_as_nat c h0 p))
 
 let lemma_point_to_domain #c h0 h1 p result = ()
 
 
-val lemma_pif_to_domain: #c: curve -> h: mem ->  p: point c -> Lemma
-  (requires (
-    point_x_as_nat c h p == 0 /\ 
-    point_y_as_nat c h p == 0 /\ 
-    point_z_as_nat c h p == 0))
-  (ensures (fromDomainPoint #c #DH
-    (point_prime_to_coordinates c (as_seq h p)) == 
-    point_prime_to_coordinates c (as_seq h p)))
+val lemma_pif_to_domain: #c: curve -> h: mem -> p: point c -> Lemma
+  (requires (point_eval c h p /\ point_x_as_nat c h p == 0 /\ point_y_as_nat c h p == 0 /\ point_z_as_nat c h p == 0))
+  (ensures (fromDomainPoint #c #DH (point_as_nat c h p) == point_as_nat c h p))
+
 
 let lemma_pif_to_domain #c h p = 
-  let (x, y, z) = point_prime_to_coordinates c (as_seq h p) in 
+  let (x, y, z) = point_as_nat c h p in 
   let (x3, y3, z3) = fromDomainPoint #c #DH (x, y, z) in 
   lemmaFromDomain #c #DH x;
   lemmaFromDomain #c #DH y;
@@ -313,8 +272,8 @@ let lemma_pif_to_domain #c h p =
   lemma_multiplication_not_mod_prime #c z
 
 
-val lemma_coord: #c: curve -> h3: mem -> q: point c -> Lemma (
-   let (r0, r1, r2) = fromDomainPoint #c #DH (point_prime_to_coordinates c (as_seq h3 q)) in 
+val lemma_coord: #c: curve -> h3: mem -> q: point c {point_eval c h3 q} -> Lemma (
+   let (r0, r1, r2) = fromDomainPoint #c #DH (point_as_nat c h3 q) in 
    let xD = fromDomain_ #c #DH (point_x_as_nat c h3 q) in 
    let yD = fromDomain_ #c #DH (point_y_as_nat c h3 q) in 
    let zD = fromDomain_ #c #DH (point_z_as_nat c h3 q) in 
@@ -323,54 +282,89 @@ val lemma_coord: #c: curve -> h3: mem -> q: point c -> Lemma (
 let lemma_coord h3 q = ()
 
 
+val uploadStartPoints: #c: curve -> q: point c -> p: point c -> result: point c -> Stack unit 
+  (requires fun h -> live h q /\ live h p /\ live h result /\ 
+    disjoint p q /\ disjoint q result /\ eq_or_disjoint p result /\ point_eval c h p /\
+    ~ (isPointAtInfinity (point_as_nat c h p)))
+  (ensures fun h0 _ h1 -> modifies (loc result |+| loc q) h0 h1 /\
+    point_eval c h1 q /\ point_eval c h1 result /\ (
+    let pD = fromDomainPoint #c #DH (point_as_nat c h1 q) in 
+    let qD = fromDomainPoint #c #DH (point_as_nat c h1 result) in 
+    qD == point_as_nat c h0 p /\ isPointAtInfinity pD /\  pointEqual #c pD (point_mult #c 0 qD) /\ ~ (pointEqual #c pD qD)))
+
+let uploadStartPoints #c q p result = 
+    let h0 = ST.get() in 
+  uploadZeroPoint #c q;
+    let h1 = ST.get() in 
+  Hacl.Impl.P.PointAdd.Aux.lemma_coord_eval c h0 h1 p;
+  pointToDomain #c p result;
+    let h2 = ST.get() in 
+  Hacl.Impl.P.PointAdd.Aux.lemma_coord_eval c h1 h2 q;
+  
+  lemma_point_to_domain h1 h2 p result;
+  lemma_pif_to_domain #c h1 q;
+
+  let qD = fromDomainPoint #c #DH (point_as_nat c h2 result) in 
+  point_mult_0 #c qD 0; 
+
+  let x, y, z = point_as_nat c h2 result in 
+  lemma_pointAtInfInDomain #c x y z
+
+
+val scalar_multiplication_t_0: #c: curve -> #t:buftype -> q: point c -> p: point c -> result: point c -> 
+  scalar: lbuffer_t t uint8 (getScalarLenBytes c) -> 
+  tempBuffer: lbuffer uint64 (size 17 *! getCoordinateLenU64 c) ->
+  Stack unit 
+  (requires fun h -> live h q /\ live h p /\ live h result /\ live h scalar /\ live h tempBuffer /\
+    LowStar.Monotonic.Buffer.all_disjoint [loc p; loc q; loc tempBuffer; loc scalar] /\
+    disjoint q result /\ eq_or_disjoint p result /\ disjoint result tempBuffer /\ disjoint result scalar /\
+    point_eval c h p /\ ~ (isPointAtInfinity (point_as_nat c h p)))
+  (ensures fun h0 _ h1 -> modifies (loc q |+| loc result |+| loc tempBuffer) h0 h1 /\ point_eval c h1 q /\ (
+    let i1 = point_as_nat c h0 p in 
+    point_mult_0 i1 0; 
+    let pD = fromDomainPoint #c #DH (point_as_nat c h1 q) in
+    let r0, r1 = montgomery_ladder_spec_left (as_seq h0 scalar) (pointAtInfinity , i1) in pointEqual pD r0))
+
+
+let scalar_multiplication_t_0 #c  q p result scalar tempBuffer = 
+    let h0 = ST.get() in 
+  uploadStartPoints q p result; 
+    let h1 = ST.get() in 
+  montgomery_ladder q result scalar tempBuffer
+
+
+val point_mult_0: #c: curve -> p: point_nat_prime #c ->  Lemma (point_mult #c 0 p == pointAtInfinity)
+
+let point_mult_0 #c p = Spec.ECC.point_mult_0 p 0
+
+
 inline_for_extraction
 val scalarMultiplication_t: #c: curve -> #t:buftype -> p: point c -> result: point c -> 
-  scalar: lbuffer_t t uint8 (getScalarLen c) -> 
+  scalar: lbuffer_t t uint8 (getScalarLenBytes c) -> 
   tempBuffer: lbuffer uint64 (size 20 *! getCoordinateLenU64 c) ->
   Stack unit
-    (requires fun h -> 
-      let len = getCoordinateLenU64 c in 
-      let prime = getPrime c in 
-      live h p /\ live h result /\ live h scalar /\ live h tempBuffer /\
-      LowStar.Monotonic.Buffer.all_disjoint [loc p; loc tempBuffer; loc scalar; loc result] /\
-      as_nat c h (gsub p (size 0) len) < prime /\ 
-      as_nat c h (gsub p len len) < prime /\
-      as_nat c h (gsub p (size 2 *! len) len) < prime 
-    )
-  (ensures fun h0 _ h1 -> 
-    let prime = getPrime c in 
-    let len = getCoordinateLenU64 c in 
-    modifies (loc p |+| loc result |+| loc tempBuffer) h0 h1  /\ 
-    
-    as_nat c h1 (gsub result (size 0) len) < prime /\ 
-    as_nat c h1 (gsub result len len) < prime /\
-    as_nat c h1 (gsub result (size 2 *! len) len) < prime /\
-    
-    modifies (loc p |+| loc result |+| loc tempBuffer) h0 h1 /\
-    (
-      let x3, y3, z3 = point_x_as_nat c h1 result, point_y_as_nat c h1 result, point_z_as_nat c h1 result in 
-      let (xN, yN, zN) = scalar_multiplication #c (as_seq h0 scalar) (point_prime_to_coordinates c (as_seq h0 p)) in 
-      x3 == xN /\ y3 == yN /\ z3 == zN 
-    ) 
-) 
+  (requires fun h -> 
+    live h p /\ live h result /\ live h scalar /\ live h tempBuffer /\
+    LowStar.Monotonic.Buffer.all_disjoint [loc p; loc tempBuffer; loc scalar; loc result] /\ point_eval c h p /\
+    ~ (isPointAtInfinity (point_as_nat c h p)))
+  (ensures fun h0 _ h1 -> modifies (loc p |+| loc result |+| loc tempBuffer) h0 h1 /\ point_eval c h1 result /\ (
+    pointEqual (scalar_multiplication (as_seq h0 scalar) (point_as_nat c h0 p)) (point_as_nat c h1 result)))
 
+val size_cuttable_scalar_mult: #c: curve -> 
+  Lemma (let len = getCoordinateLenU64 c in  (v (size 3 *! len) + v (size 17 *! len) <= v (size 20 *! len)))
+
+let size_cuttable_scalar_mult #c = ()
 
 let scalarMultiplication_t #c #t p result scalar tempBuffer  = 
     let h0 = ST.get() in 
   let len = getCoordinateLenU64 c in 
   let q = sub tempBuffer (size 0) (size 3 *! len) in 
-  uploadZeroPoint #c q;
-  let buff = sub tempBuffer (size 3 *! len) (size 22 *! len) in 
-  pointToDomain p result;
-    let h2 = ST.get() in 
-  montgomery_ladder q result scalar buff;
-    admit();
-    let h3 = ST.get() in 
-    lemma_point_to_domain h0 h2 p result;
-    lemma_pif_to_domain #c h2 q;
+  size_cuttable_scalar_mult #c;
+  let buff = sub tempBuffer (size 3 *! len) (size 17 *! len) in
+  scalar_multiplication_t_0 q p result scalar buff; 
   norm q result buff; 
-    lemma_coord #c  h3 q;
-    admit()
+  let i1 = point_as_nat c h0 p in 
+    point_mult_0 i1
 
 
 let scalarMultiplicationL #c = scalarMultiplication_t #c #MUT
@@ -383,87 +377,6 @@ let scalarMultiplication #c #buf_type p result scalar tempBuffer =
   |MUT -> scalarMultiplicationL #c p result scalar tempBuffer 
   |IMMUT -> scalarMultiplicationI #c p result scalar tempBuffer
   |CONST -> scalarMultiplicationC #c p result scalar tempBuffer
-
-
-val uploadBasePoint: #c: curve -> p: point c -> Stack unit 
-  (requires fun h -> live h p)
-  (ensures fun h0 _ h1 -> 
-    let len = getCoordinateLenU64 c in 
-    let prime = getPrime c in 
-  
-    modifies (loc p) h0 h1 /\ 
-    as_nat c h1 (gsub p (size 0) len) < prime /\ 
-    as_nat c h1 (gsub p len len) < prime /\
-    as_nat c h1 (gsub p (size 2 *! len) len) < prime /\ (
-    
-    let x1 = as_nat c h1 (gsub p (size 0) len) in 
-    let y1 = as_nat c h1 (gsub p len len) in 
-    let z1 = as_nat c h1 (gsub p (size 2 *! len) len) in 
-
-    let baseX, baseY, baseZ = basePoint #c in 
-    fromDomain_ #c #DH x1 == baseX /\ fromDomain_ #c #DH y1 == baseY /\ fromDomain_ #c #DH z1 == baseZ))
-
-let uploadBasePoint #c p = 
-  match c with
-  |P384 -> 
-    let h0 = ST.get() in
-    upd p (size 0) (u64 0x3dd0756649c0b528);
-    upd p (size 1) (u64 0x20e378e2a0d6ce38);
-    upd p (size 2) (u64 0x879c3afc541b4d6e);
-    upd p (size 3) (u64 0x6454868459a30eff);
-    upd p (size 4) (u64 0x812ff723614ede2b);
-    upd p (size 5) (u64 0x4d3aadc2299e1513);
-
-
-    upd p (size 6) (u64 0x23043dad4b03a4fe);
-    upd p (size 7) (u64 0xa1bfa8bf7bb4a9ac);
-    upd p (size 8) (u64 0x8bade7562e83b050);
-    upd p (size 9) (u64 0xc6c3521968f4ffd9);
-    upd p (size 10) (u64 0xdd8002263969a840);
-    upd p (size 11) (u64 0x2b78abc25a15c5e9);
-
-    upd p (size 12) (u64 0xffffffff00000001);
-    upd p (size 13) (u64 0xffffffff);
-    upd p (size 14) (u64 0x1);
-    upd p (size 15) (u64 0);
-    upd p (size 16) (u64 0);
-    upd p (size 17) (u64 0);
-    admit()
-
-
-
-  |P256 -> 
-    let h0 = ST.get() in 
-  upd p (size 0) (u64 0x79e730d418a9143c);
-  upd p (size 1) (u64 0x75ba95fc5fedb601);
-  upd p (size 2) (u64 0x79fb732b77622510);
-  upd p (size 3) (u64 0x18905f76a53755c6);
-
-(*
-  assert_norm (8784043285714375740 + pow2 64 * 8483257759279461889 + pow2 64 * pow2 64 * 8789745728267363600 + pow2 64 * pow2 64 * pow2 64 * 1770019616739251654 < prime256); 
-    assert_norm (8784043285714375740 + pow2 64 * 8483257759279461889 + pow2 64 * pow2 64 * 8789745728267363600 + pow2 64 * pow2 64 * pow2 64 * 1770019616739251654 = 11110593207902424140321080247206512405358633331993495164878354046817554469948); 
-  assert_norm(0x6B17D1F2E12C4247F8BCE6E563A440F277037D812DEB33A0F4A13945D898C296 == fromDomain #P256 11110593207902424140321080247206512405358633331993495164878354046817554469948);
-*) 
-  upd p (size 4) (u64 0xddf25357ce95560a);
-  upd p (size 5) (u64 0x8b4ab8e4ba19e45c);
-  upd p (size 6) (u64 0xd2e88688dd21f325);
-  upd p (size 7) (u64 0x8571ff1825885d85);
-(* 
-  assert_norm(15992936863339206154 + pow2 64 * 10037038012062884956 + pow2 64 * pow2 64 * 15197544864945402661 + pow2 64 * pow2 64 * pow2 64 * 9615747158586711429 < prime256);
-  assert_norm (15992936863339206154 + pow2 64 * 10037038012062884956 + pow2 64 * pow2 64 * 15197544864945402661 + pow2 64 * pow2 64 * pow2 64 * 9615747158586711429 = 60359023176204190920225817201443260813112970217682417638161152432929735267850);
-  assert_norm (0x4FE342E2FE1A7F9B8EE7EB4A7C0F9E162BCE33576B315ECECBB6406837BF51F5 == fromDomain #P256 60359023176204190920225817201443260813112970217682417638161152432929735267850);
-  *)
-  
-  upd p (size 8) (u64 0x1);
-  upd p (size 9) (u64 0xffffffff00000000);
-  upd p (size 10) (u64 0xffffffffffffffff);
-  upd p (size 11) (u64 0xfffffffe);
-  
-  (* 
-  assert_norm (1 + pow2 64 * 18446744069414584320 + pow2 64 * pow2 64 * 18446744073709551615 + pow2 64 * pow2 64 * pow2 64 * 4294967294 < prime256);
-  assert_norm (1 = fromDomain #P256 26959946660873538059280334323183841250350249843923952699046031785985);
-  assert_norm (1 + pow2 64 * 18446744069414584320 + pow2 64 * pow2 64 * 18446744073709551615 + pow2 64 * pow2 64 * pow2 64 * 4294967294 = 26959946660873538059280334323183841250350249843923952699046031785985)  *)
-  admit()
 
 
 let scalarMultiplicationWithoutNorm #c p result scalar tempBuffer = 
